02Typed/Type.thy
@@ -3,32 +3,7 @@ theory Type
 begin
 
 datatype ty = 
-  TyVar var
-  | Num 
+  Num 
   | Arrow ty ty
-
-primrec tvars :: "ty \<Rightarrow> var set" where
-  "tvars (TyVar y) = {y}"
-| "tvars Num = {}"
-| "tvars (Arrow t\<^sub>1 t\<^sub>2) = tvars t\<^sub>1 \<union> tvars t\<^sub>2"
-
-fun tsubst :: "var \<Rightarrow> ty \<Rightarrow> ty \<Rightarrow> ty" where
-  "tsubst x t' (TyVar y) = (if x = y then t' else TyVar y)"
-| "tsubst x t' Num = Num"
-| "tsubst x t' (Arrow t\<^sub>1 t\<^sub>2) = Arrow (tsubst x t' t\<^sub>1) (tsubst x t' t\<^sub>2)"
-
-lemma [simp]: "x \<notin> tvars t \<Longrightarrow> tsubst x t' t = t"
-  by (induction t) simp_all
-
-lemma [simp]: "tsubst x (TyVar x) t = t"
-  by (induction t) simp_all
-
-lemma [simp]: "y \<notin> tvars t \<Longrightarrow> tsubst y t' (tsubst x (TyVar y) t) = tsubst x t' t"
-  by (induction t) simp_all
-
-lemma tsubst_arrow [consumes 1, case_names TyVar Arrow]: "Arrow t\<^sub>1 t\<^sub>2 = tsubst y t' tt \<Longrightarrow> 
-  (t' = Arrow t\<^sub>1 t\<^sub>2 \<Longrightarrow> tt = TyVar y \<Longrightarrow> P) \<Longrightarrow> 
-    (\<And>tt\<^sub>1 tt\<^sub>2. t\<^sub>1 = tsubst y t' tt\<^sub>1 \<Longrightarrow> t\<^sub>2 = tsubst y t' tt\<^sub>2 \<Longrightarrow> tt = Arrow tt\<^sub>1 tt\<^sub>2 \<Longrightarrow> P) \<Longrightarrow> P"
-  by (induction tt) (simp_all split: if_splits)
 
 end
