Readme.md
@@ -14,3 +14,4 @@ Refactorings:
 
 - constr_subst -> full substitution?
 - Make contraint functions use list functions?
+- Make map functions on expr\s use actual map
